improve readability of extracted add1sp1

code/mpfr/injected/add1sp1_extracted.c
@@ -57,8 +57,6 @@ typedef struct K___uint64_t_uint64_t_int64_t_s
 K___uint64_t_uint64_t_int64_t;
 
 #define MPFR_Lib_mpfr_struct __mpfr_struct
-#define MPFR_Lib_mpfr_RET(I) ((I) != 0 ? ((__gmpfr_flags |= MPFR_FLAGS_INEXACT), (I)) : 0)
-#define MPFR_Exceptions_mpfr_overflow mpfr_overflow
 #define mpfr_prec _mpfr_prec
 #define mpfr_exp _mpfr_exp
 #define mpfr_d _mpfr_d
@@ -66,30 +64,31 @@ K___uint64_t_uint64_t_int64_t;
 #define MPFR_Lib_gmp_NUMB_BITS GMP_NUMB_BITS
 #define MPFR_Lib_mpfr_EMAX __gmpfr_emax
 
-#define MPFR_RoundingMode_uu___is_MPFR_RNDN(rnd_mode) (rnd_mode == MPFR_RNDN)
+#define MPFR_Lib_mpfr_SET_EXP MPFR_SET_EXP
+#define MPFR_Exceptions_mpfr_overflow mpfr_overflow
 #define MPFR_RoundingMode_mpfr_IS_LIKE_RNDZ MPFR_IS_LIKE_RNDZ
 
-/* same as mpfr_add1sp, but for p < GMP_NUMB_BITS */
+#define MPFR_Lib_mpfr_NEG_SIGN(s) (-(s))
+#define MPFR_Lib_mpfr_RET(I) ((I) != 0 ? ((__gmpfr_flags |= MPFR_FLAGS_INEXACT), (I)) : 0)
+#define MPFR_RoundingMode_uu___is_MPFR_RNDN(rnd_mode) (rnd_mode == MPFR_RNDN)
+
 static int
 mpfr_add1sp1 (mpfr_ptr a, mpfr_srcptr b, mpfr_srcptr c, mpfr_rnd_t rnd_mode,
               mpfr_prec_t p)
 {
-  MPFR_Lib_mpfr_struct a0 = a[0U];
-  MPFR_Lib_mpfr_struct b0 = b[0U];
-  MPFR_Lib_mpfr_struct c0 = c[0U];
-  int64_t bx = b0.mpfr_exp;
-  int64_t cx = c0.mpfr_exp;
+  int64_t bx = b->mpfr_exp;
+  int64_t cx = c->mpfr_exp;
+  uint64_t *ap0 = a->mpfr_d;
+  uint64_t *bp = b->mpfr_d;
+  uint64_t *cp = c->mpfr_d;
   int64_t sh = MPFR_Lib_gmp_NUMB_BITS - p;
   MPFR_Add1sp1_state st;
   if (bx == cx)
   {
-    uint64_t *ap = a0.mpfr_d;
-    uint64_t *bp = b0.mpfr_d;
-    uint64_t *cp = c0.mpfr_d;
-    uint64_t a01 = (bp[0U] >> (uint32_t)1U) + (cp[0U] >> (uint32_t)1U);
-    int64_t bx1 = b0.mpfr_exp + (int64_t)1;
-    uint64_t rb = a01 & (uint64_t)1U << (uint32_t)(sh - (int64_t)1);
-    ap[0U] = a01 ^ rb;
+    uint64_t a0 = (bp[0U] >> (uint32_t)1U) + (cp[0U] >> (uint32_t)1U);
+    int64_t bx1 = bx + (int64_t)1;
+    uint64_t rb = a0 & (uint64_t)1U << (uint32_t)(sh - (int64_t)1);
+    ap0[0U] = a0 ^ rb;
     uint64_t sb = (uint64_t)0U;
     st = MPFR_Add1sp1_mk_state(sh, bx1, rb, sb);
   }
@@ -98,76 +97,63 @@ mpfr_add1sp1 (mpfr_ptr a, mpfr_srcptr b, mpfr_srcptr c, mpfr_rnd_t rnd_mode,
     MPFR_Add1sp1_state ite0;
     if (bx > cx)
     {
-      int64_t bx1 = b0.mpfr_exp;
-      int64_t cx1 = c0.mpfr_exp;
-      int64_t d = bx1 - cx1;
+      int64_t d = bx - cx;
       uint64_t mask = ((uint64_t)1U << (uint32_t)sh) - (uint64_t)1U;
       MPFR_Add1sp1_state ite1;
       if (d < sh)
       {
-        uint64_t *ap = a0.mpfr_d;
-        uint64_t *bp = b0.mpfr_d;
-        uint64_t *cp = c0.mpfr_d;
-        int64_t bx2 = b0.mpfr_exp;
-        uint64_t a01 = bp[0U] + (cp[0U] >> (uint32_t)d);
+        uint64_t a0 = bp[0U] + (cp[0U] >> (uint32_t)d);
         K___uint64_t_int64_t scrut;
-        if (a01 < bp[0U])
+        if (a0 < bp[0U])
           scrut =
             (
               (K___uint64_t_int64_t){
-                .fst = (uint64_t)0x8000000000000000U | a01 >> (uint32_t)1U,
-                .snd = bx2 + (int64_t)1
+                .fst = (uint64_t)0x8000000000000000U | a0 >> (uint32_t)1U,
+                .snd = bx + (int64_t)1
               }
             );
         else
-          scrut = ((K___uint64_t_int64_t){ .fst = a01, .snd = bx2 });
-        uint64_t a02 = scrut.fst;
-        int64_t bx3 = scrut.snd;
-        uint64_t rb = a02 & (uint64_t)1U << (uint32_t)(sh - (int64_t)1);
-        uint64_t sb = (a02 & mask) ^ rb;
-        ap[0U] = a02 & ~mask;
-        ite1 = MPFR_Add1sp1_mk_state(sh, bx3, rb, sb);
+          scrut = ((K___uint64_t_int64_t){ .fst = a0, .snd = bx });
+        uint64_t a01 = scrut.fst;
+        int64_t bx1 = scrut.snd;
+        uint64_t rb = a01 & (uint64_t)1U << (uint32_t)(sh - (int64_t)1);
+        uint64_t sb = (a01 & mask) ^ rb;
+        ap0[0U] = a01 & ~mask;
+        ite1 = MPFR_Add1sp1_mk_state(sh, bx1, rb, sb);
       }
       else
       {
         MPFR_Add1sp1_state ite;
         if (d < MPFR_Lib_gmp_NUMB_BITS)
         {
-          uint64_t *ap = a0.mpfr_d;
-          uint64_t *bp = b0.mpfr_d;
-          uint64_t *cp = c0.mpfr_d;
-          int64_t bx2 = b0.mpfr_exp;
           uint64_t sb = cp[0U] << (uint32_t)(MPFR_Lib_gmp_NUMB_BITS - d);
-          uint64_t a01 = bp[0U] + (cp[0U] >> (uint32_t)d);
+          uint64_t a0 = bp[0U] + (cp[0U] >> (uint32_t)d);
           K___uint64_t_uint64_t_int64_t scrut;
-          if (a01 < bp[0U])
+          if (a0 < bp[0U])
             scrut =
               (
                 (K___uint64_t_uint64_t_int64_t){
-                  .fst = sb | (a01 & (uint64_t)1U),
-                  .snd = (uint64_t)0x8000000000000000U | a01 >> (uint32_t)1U,
-                  .thd = bx2 + (int64_t)1
+                  .fst = sb | (a0 & (uint64_t)1U),
+                  .snd = (uint64_t)0x8000000000000000U | a0 >> (uint32_t)1U,
+                  .thd = bx + (int64_t)1
                 }
               );
           else
-            scrut = ((K___uint64_t_uint64_t_int64_t){ .fst = sb, .snd = a01, .thd = bx2 });
+            scrut = ((K___uint64_t_uint64_t_int64_t){ .fst = sb, .snd = a0, .thd = bx });
           uint64_t sb1 = scrut.fst;
-          uint64_t a02 = scrut.snd;
-          int64_t bx3 = scrut.thd;
-          uint64_t rb = a02 & (uint64_t)1U << (uint32_t)(sh - (int64_t)1);
-          uint64_t sb2 = sb1 | ((a02 & mask) ^ rb);
-          ap[0U] = a02 & ~mask;
-          ite = MPFR_Add1sp1_mk_state(sh, bx3, rb, sb2);
+          uint64_t a01 = scrut.snd;
+          int64_t bx1 = scrut.thd;
+          uint64_t rb = a01 & (uint64_t)1U << (uint32_t)(sh - (int64_t)1);
+          uint64_t sb2 = sb1 | ((a01 & mask) ^ rb);
+          ap0[0U] = a01 & ~mask;
+          ite = MPFR_Add1sp1_mk_state(sh, bx1, rb, sb2);
         }
         else
         {
-          uint64_t *ap = a0.mpfr_d;
-          uint64_t *bp = b0.mpfr_d;
-          int64_t bx2 = b0.mpfr_exp;
-          ap[0U] = bp[0U];
+          ap0[0U] = bp[0U];
           uint64_t rb = (uint64_t)0U;
           uint64_t sb = (uint64_t)1U;
-          ite = MPFR_Add1sp1_mk_state(sh, bx2, rb, sb);
+          ite = MPFR_Add1sp1_mk_state(sh, bx, rb, sb);
         }
         ite1 = ite;
       }
@@ -175,76 +161,63 @@ mpfr_add1sp1 (mpfr_ptr a, mpfr_srcptr b, mpfr_srcptr c, mpfr_rnd_t rnd_mode,
     }
     else
     {
-      int64_t bx1 = c0.mpfr_exp;
-      int64_t cx1 = b0.mpfr_exp;
-      int64_t d = bx1 - cx1;
+      int64_t d = cx - bx;
       uint64_t mask = ((uint64_t)1U << (uint32_t)sh) - (uint64_t)1U;
       MPFR_Add1sp1_state ite1;
       if (d < sh)
       {
-        uint64_t *ap = a0.mpfr_d;
-        uint64_t *bp = c0.mpfr_d;
-        uint64_t *cp = b0.mpfr_d;
-        int64_t bx2 = c0.mpfr_exp;
-        uint64_t a01 = bp[0U] + (cp[0U] >> (uint32_t)d);
+        uint64_t a0 = cp[0U] + (bp[0U] >> (uint32_t)d);
         K___uint64_t_int64_t scrut;
-        if (a01 < bp[0U])
+        if (a0 < cp[0U])
           scrut =
             (
               (K___uint64_t_int64_t){
-                .fst = (uint64_t)0x8000000000000000U | a01 >> (uint32_t)1U,
-                .snd = bx2 + (int64_t)1
+                .fst = (uint64_t)0x8000000000000000U | a0 >> (uint32_t)1U,
+                .snd = cx + (int64_t)1
               }
             );
         else
-          scrut = ((K___uint64_t_int64_t){ .fst = a01, .snd = bx2 });
-        uint64_t a02 = scrut.fst;
-        int64_t bx3 = scrut.snd;
-        uint64_t rb = a02 & (uint64_t)1U << (uint32_t)(sh - (int64_t)1);
-        uint64_t sb = (a02 & mask) ^ rb;
-        ap[0U] = a02 & ~mask;
-        ite1 = MPFR_Add1sp1_mk_state(sh, bx3, rb, sb);
+          scrut = ((K___uint64_t_int64_t){ .fst = a0, .snd = cx });
+        uint64_t a01 = scrut.fst;
+        int64_t bx1 = scrut.snd;
+        uint64_t rb = a01 & (uint64_t)1U << (uint32_t)(sh - (int64_t)1);
+        uint64_t sb = (a01 & mask) ^ rb;
+        ap0[0U] = a01 & ~mask;
+        ite1 = MPFR_Add1sp1_mk_state(sh, bx1, rb, sb);
       }
       else
       {
         MPFR_Add1sp1_state ite;
         if (d < MPFR_Lib_gmp_NUMB_BITS)
         {
-          uint64_t *ap = a0.mpfr_d;
-          uint64_t *bp = c0.mpfr_d;
-          uint64_t *cp = b0.mpfr_d;
-          int64_t bx2 = c0.mpfr_exp;
-          uint64_t sb = cp[0U] << (uint32_t)(MPFR_Lib_gmp_NUMB_BITS - d);
-          uint64_t a01 = bp[0U] + (cp[0U] >> (uint32_t)d);
+          uint64_t sb = bp[0U] << (uint32_t)(MPFR_Lib_gmp_NUMB_BITS - d);
+          uint64_t a0 = cp[0U] + (bp[0U] >> (uint32_t)d);
           K___uint64_t_uint64_t_int64_t scrut;
-          if (a01 < bp[0U])
+          if (a0 < cp[0U])
             scrut =
               (
                 (K___uint64_t_uint64_t_int64_t){
-                  .fst = sb | (a01 & (uint64_t)1U),
-                  .snd = (uint64_t)0x8000000000000000U | a01 >> (uint32_t)1U,
-                  .thd = bx2 + (int64_t)1
+                  .fst = sb | (a0 & (uint64_t)1U),
+                  .snd = (uint64_t)0x8000000000000000U | a0 >> (uint32_t)1U,
+                  .thd = cx + (int64_t)1
                 }
               );
           else
-            scrut = ((K___uint64_t_uint64_t_int64_t){ .fst = sb, .snd = a01, .thd = bx2 });
+            scrut = ((K___uint64_t_uint64_t_int64_t){ .fst = sb, .snd = a0, .thd = cx });
           uint64_t sb1 = scrut.fst;
-          uint64_t a02 = scrut.snd;
-          int64_t bx3 = scrut.thd;
-          uint64_t rb = a02 & (uint64_t)1U << (uint32_t)(sh - (int64_t)1);
-          uint64_t sb2 = sb1 | ((a02 & mask) ^ rb);
-          ap[0U] = a02 & ~mask;
-          ite = MPFR_Add1sp1_mk_state(sh, bx3, rb, sb2);
+          uint64_t a01 = scrut.snd;
+          int64_t bx1 = scrut.thd;
+          uint64_t rb = a01 & (uint64_t)1U << (uint32_t)(sh - (int64_t)1);
+          uint64_t sb2 = sb1 | ((a01 & mask) ^ rb);
+          ap0[0U] = a01 & ~mask;
+          ite = MPFR_Add1sp1_mk_state(sh, bx1, rb, sb2);
         }
         else
         {
-          uint64_t *ap = a0.mpfr_d;
-          uint64_t *bp = c0.mpfr_d;
-          int64_t bx2 = c0.mpfr_exp;
-          ap[0U] = bp[0U];
+          ap0[0U] = cp[0U];
           uint64_t rb = (uint64_t)0U;
           uint64_t sb = (uint64_t)1U;
-          ite = MPFR_Add1sp1_mk_state(sh, bx2, rb, sb);
+          ite = MPFR_Add1sp1_mk_state(sh, cx, rb, sb);
         }
         ite1 = ite;
       }
@@ -260,17 +233,8 @@ mpfr_add1sp1 (mpfr_ptr a, mpfr_srcptr b, mpfr_srcptr c, mpfr_rnd_t rnd_mode,
   else
   {
     uint64_t *ap = a->mpfr_d;
-    uint64_t a01 = ap[0U];
-    MPFR_Lib_mpfr_struct uu___72_3478 = a[0U];
-    a[0U] =
-      (
-        (MPFR_Lib_mpfr_struct){
-          .mpfr_prec = uu___72_3478.mpfr_prec,
-          .mpfr_sign = uu___72_3478.mpfr_sign,
-          .mpfr_exp = st.bx,
-          .mpfr_d = uu___72_3478.mpfr_d
-        }
-      );
+    uint64_t a0 = ap[0U];
+    MPFR_Lib_mpfr_SET_EXP(a, st.bx);
     if (st.rb == (uint64_t)0U && st.sb == (uint64_t)0U)
       return MPFR_Lib_mpfr_RET((int32_t)0);
     else if (MPFR_RoundingMode_uu___is_MPFR_RNDN(rnd_mode))
@@ -278,16 +242,9 @@ mpfr_add1sp1 (mpfr_ptr a, mpfr_srcptr b, mpfr_srcptr c, mpfr_rnd_t rnd_mode,
       (
         st.rb
         == (uint64_t)0U
-        || (st.sb == (uint64_t)0U && (a01 & (uint64_t)1U << (uint32_t)st.sh) == (uint64_t)0U)
+        || (st.sb == (uint64_t)0U && (a0 & (uint64_t)1U << (uint32_t)st.sh) == (uint64_t)0U)
       )
-      {
-        int32_t ite;
-        if (a->mpfr_sign == (int32_t)1)
-          ite = (int32_t)-1;
-        else
-          ite = (int32_t)1;
-        return MPFR_Lib_mpfr_RET(ite);
-      }
+        return MPFR_Lib_mpfr_RET(MPFR_Lib_mpfr_NEG_SIGN(a->mpfr_sign));
       else
       {
         uint64_t *ap1 = a->mpfr_d;
@@ -297,16 +254,7 @@ mpfr_add1sp1 (mpfr_ptr a, mpfr_srcptr b, mpfr_srcptr c, mpfr_rnd_t rnd_mode,
           ap1[0U] = (uint64_t)0x8000000000000000U;
           if (st.bx + (int64_t)1 <= MPFR_Lib_mpfr_EMAX)
           {
-            MPFR_Lib_mpfr_struct uu___72_3574 = a[0U];
-            a[0U] =
-              (
-                (MPFR_Lib_mpfr_struct){
-                  .mpfr_prec = uu___72_3574.mpfr_prec,
-                  .mpfr_sign = uu___72_3574.mpfr_sign,
-                  .mpfr_exp = st.bx + (int64_t)1,
-                  .mpfr_d = uu___72_3574.mpfr_d
-                }
-              );
+            MPFR_Lib_mpfr_SET_EXP(a, st.bx + (int64_t)1);
             return MPFR_Lib_mpfr_RET(a->mpfr_sign);
           }
           else
@@ -319,14 +267,7 @@ mpfr_add1sp1 (mpfr_ptr a, mpfr_srcptr b, mpfr_srcptr c, mpfr_rnd_t rnd_mode,
           return MPFR_Lib_mpfr_RET(a->mpfr_sign);
       }
     else if (MPFR_RoundingMode_mpfr_IS_LIKE_RNDZ(rnd_mode, a->mpfr_sign < (int32_t)0))
-    {
-      int32_t ite;
-      if (a->mpfr_sign == (int32_t)1)
-        ite = (int32_t)-1;
-      else
-        ite = (int32_t)1;
-      return MPFR_Lib_mpfr_RET(ite);
-    }
+      return MPFR_Lib_mpfr_RET(MPFR_Lib_mpfr_NEG_SIGN(a->mpfr_sign));
     else
     {
       uint64_t *ap1 = a->mpfr_d;
@@ -336,16 +277,7 @@ mpfr_add1sp1 (mpfr_ptr a, mpfr_srcptr b, mpfr_srcptr c, mpfr_rnd_t rnd_mode,
         ap1[0U] = (uint64_t)0x8000000000000000U;
         if (st.bx + (int64_t)1 <= MPFR_Lib_mpfr_EMAX)
         {
-          MPFR_Lib_mpfr_struct uu___72_3781 = a[0U];
-          a[0U] =
-            (
-              (MPFR_Lib_mpfr_struct){
-                .mpfr_prec = uu___72_3781.mpfr_prec,
-                .mpfr_sign = uu___72_3781.mpfr_sign,
-                .mpfr_exp = st.bx + (int64_t)1,
-                .mpfr_d = uu___72_3781.mpfr_d
-              }
-            );
+          MPFR_Lib_mpfr_SET_EXP(a, st.bx + (int64_t)1);
           return MPFR_Lib_mpfr_RET(a->mpfr_sign);
         }
         else
